\begin{enumerate}
\item 
Students will probably find $\mu(t)=e^t$, but we can take $\mu(t)=5e^t$ or really any other constant multiple. The integrating factor is only unique up to a constant.

\item 
\begin{enumerate}
    \item 
    $y=1$ is semistable,
    $y=2$ is stable,
    $y=3$ is unstable
    
    A visual argument (``If we are just below 1, the derivative is positive, so it's going back to 1'') is nicer than an abstract argument that seems memorized (``If the phase plot crosses from top left to bottom right, it is stable'')

    \item 
    At $y=2.8$, the derivative is negative. The function will decrease. It will continue to do so until $y$ is getting close to 2. The limit will be 2.
\end{enumerate}

    \item 
    We can substitute $z = \frac{dy}{dx}$ in order to convert the ODE into a first-order one:
	        \[
	            \sqrt{1 + z^2} = x\frac{dz}{dx}\\
	        \]
	        This is a separable ODE, so we can write it as:
	        \[
	            \frac{dz}{\sqrt{1+z^2}} = \frac{dx}{x}\\
	            \int\frac{dz}{\sqrt{1+z^2}} = \int\frac{dx}{x}\\
	        \]
	        The integral on the left can be solved by using the trigonometric substitution $z = \tan{\theta}, dz = \sec^2{\theta}d\theta$.
	        
	        \[
	            \int\frac{\sec^2{\theta}d\theta}{\sec{\theta}}\\
	            = \int\sec{\theta}d\theta\\
	            = \ln|\sec{\theta} + \tan{\theta}| + C\\
	            = \ln{\left|\sqrt{z^2+1} + z\right|} + C\\
	            = \ln{\left(\sqrt{z^2+1} + z\right)} + C
	        \]
	        
	        The last step is possible since $\sqrt{z^2+1} > |z| \implies \sqrt{z^2 + 1} + z > 0$.
	        The ODE then becomes:
	        \[
	            \ln{\left(\sqrt{z^2+1} + z\right)} = \ln x + D\\
	            \sqrt{z^2+1} + z = Ax\\
	            z = \frac{A^2x^2-1}{2Ax}
	        \]
	        
	        Since the tiger is initially facing the gazelle, we require $z(L)=0$, i.e., the slope of the trajectory is 0 at the tiger's initial position. We can then solve for the constant of integration $A$:
	        
	        \[
	            z(L) = 0 = \frac{A^2L^2-1}{2AL} \implies A=\frac{1}{L}
	        \]
	        
	        Substituting this into our expression for $z$, we get:
	        
	        \[
	            z = \frac{\frac{x^2}{L^2} - 1}{2\frac{x}{L}}\\
	            = \frac{1}{2L}x - \frac{L}{2x}
	        \]
	        
	        Since we are interested in the trajectory of the tiger, we must solve for $y(x)$. Hence, we integrate $z$:
	        
	        \[
	            y = \int zdx\\
	            = \frac{1}{4L}x^2 - \frac{L}{2}\ln{x} + E
	        \]
	        
	        The tiger starts at a position $(L, 0)$, so the initial condition is $y(L) = 0$:
	        
	        \[
	            0 = \frac{L^2}{4L} - \frac{L}{2}\ln{L} + E\\
	            E = \frac{L}{2}\ln{L} - \frac{L}{4}
	        \]
	        
	        The final expression for $y(x)$ is then given by:
	        
	        \[
	            y(x) = \frac{1}{4L}x^2 - \frac{L}{2}\ln{x} + \frac{L}{2}\ln{L} - \frac{L}{4}
	        \]
\end{enumerate}